alpha-rename
git-svn-id: https://projects.brucker.ch/hol-testgen/svn/HOL-TestGen/trunk/hol-testgen@11939 3260e6d1-4efc-4170-b0a7-36055960796d

src/compiler_generic/Static.thy
@@ -3,6 +3,7 @@
  *                       for the OMG Standard.
  *                       http://www.brucker.ch/projects/hol-testgen/
  *
+ * Static.thy ---
  * This file is part of HOL-TestGen.
  *
  * Copyright (c) 2013-2015 Université Paris-Sud, France
@@ -40,39 +41,32 @@
  ******************************************************************************)
 (* $Id:$ *)
 
-session "Meta_Isabelle" = HOL +
-  description {* Meta_Isabelle *}
-  options [document = pdf, document_output = document_generated]
-  theories [document = false]
-    "~~/src/HOL/Library/Code_Char"
-    "isabelle_home/src/HOL/Isabelle_Main0"
-    "isabelle_home/src/HOL/Isabelle_Main1"
-  theories
-    "meta_isabelle/Parser_Pure"
-    "meta_isabelle/Meta_Isabelle"
-    "meta_isabelle/Printer_Isabelle"
-  document_files
-    "hol-ocl-isar.sty"
-    "lstisar.sty"
-    "root.bib"
-    "root.tex"
+header{* Part ... *}
 
-session "Toy_Example" = Meta_Isabelle +
-  description {* Toy_Example *}
-  options [document = pdf, document_output = document_generated]
-  theories [document = false]
-    "~~/src/HOL/Library/List_lexord"
-    "~~/src/HOL/Library/RBT"
-    "isabelle_home/src/HOL/Isabelle_Main2"
-  theories
-    "toy_example/embedding/Generator_static"
-    "document/Rail"
-    (*"toy_example/generator/Analysis_deep"*)
-    "toy_example/generator/Analysis_shallow"
-    (*"toy_example/generator/Design_deep"*)
-    "toy_example/generator/Design_shallow"
-  document_files
-    "hol-ocl-isar.sty"
-    "lstisar.sty"
-    "root.bib"
-    "root.tex"
+theory Static
+imports Main
+begin
+
+locale L
+begin
+definition map where "map f l = rev (foldl (\<lambda>l x. f x # l) [] l)"
+definition "flatten l = foldl (\<lambda>acc l. foldl (\<lambda>acc x. x # acc) acc (rev l)) [] (rev l)"
+end
+
+lemmas [code] =
+  (*def*)
+  L.map_def
+  L.flatten_def
+
+(* *)
+
+definition "map_of_list = (foldl ((\<lambda>map. (\<lambda>(x , l1). (case (map (x)) of None \<Rightarrow> (map (x \<mapsto> l1))
+    | Some l0 \<Rightarrow> (map (x \<mapsto> (L.flatten ([l0 , l1])))))))) (Map.empty))"
+
+definition "choose_0 = fst"
+definition "choose_1 = snd"
+
+definition "deref_assocs_list to_from oid S =
+  L.flatten (L.map (choose_1 o to_from) (filter (\<lambda>p. List.member (choose_0 (to_from p)) oid) S))"
+
+end
