src/compiler_generic/toy_example/embedding/Init_rbt.thy
@@ -3,6 +3,7 @@
  *                       for the OMG Standard.
  *                       http://www.brucker.ch/projects/hol-testgen/
  *
+ * Init_rbt.thy ---
  * This file is part of HOL-TestGen.
  *
  * Copyright (c) 2013-2015 Université Paris-Sud, France
@@ -40,39 +41,46 @@
  ******************************************************************************)
 (* $Id:$ *)
 
-session "Meta_Isabelle" = HOL +
-  description {* Meta_Isabelle *}
-  options [document = pdf, document_output = document_generated]
-  theories [document = false]
-    "~~/src/HOL/Library/Code_Char"
-    "isabelle_home/src/HOL/Isabelle_Main0"
-    "isabelle_home/src/HOL/Isabelle_Main1"
-  theories
-    "meta_isabelle/Parser_Pure"
-    "meta_isabelle/Meta_Isabelle"
-    "meta_isabelle/Printer_Isabelle"
-  document_files
-    "hol-ocl-isar.sty"
-    "lstisar.sty"
-    "root.bib"
-    "root.tex"
+header{* Part ... *}
 
-session "Toy_Example" = Meta_Isabelle +
-  description {* Toy_Example *}
-  options [document = pdf, document_output = document_generated]
-  theories [document = false]
-    "~~/src/HOL/Library/List_lexord"
-    "~~/src/HOL/Library/RBT"
-    "isabelle_home/src/HOL/Isabelle_Main2"
-  theories
-    "toy_example/embedding/Generator_static"
-    "document/Rail"
-    (*"toy_example/generator/Analysis_deep"*)
-    "toy_example/generator/Analysis_shallow"
-    (*"toy_example/generator/Design_deep"*)
-    "toy_example/generator/Design_shallow"
-  document_files
-    "hol-ocl-isar.sty"
-    "lstisar.sty"
-    "root.bib"
-    "root.tex"
+theory Init_rbt
+imports "../../Init"
+        "~~/src/HOL/Library/RBT"
+        "~~/src/HOL/Library/Char_ord"
+        "~~/src/HOL/Library/List_lexord"
+begin
+
+subsection{* RBT Miscellaneous *}
+
+locale RBT
+begin
+definition "modify_def v k f rbt =
+  (case RBT.lookup rbt k of None \<Rightarrow> RBT.insert k (f v) rbt
+                      | Some _ \<Rightarrow> RBT.map_entry k f rbt)"
+definition "lookup2 rbt = (\<lambda>(x1, x2). Option.bind (RBT.lookup rbt x1) (\<lambda>rbt. RBT.lookup rbt x2))"
+definition "insert2 = (\<lambda>(x1, x2) v. RBT.modify_def RBT.empty x1 (RBT.insert x2 v))"
+end
+lemmas [code] =
+  (*def*)
+  RBT.modify_def_def
+  RBT.lookup2_def
+  RBT.insert2_def
+
+context L
+begin
+definition "unique f l = List.map_filter id (fst
+  (mapM
+    (\<lambda> (cpt, v) rbt. 
+      let f_cpt = f cpt in
+      if RBT.lookup rbt f_cpt = None then
+        (Some (cpt, v), RBT.insert f_cpt () rbt)
+      else 
+        (None, rbt))
+    l
+    RBT.empty))"
+end
+lemmas [code] =
+  (*def*)
+  L.unique_def
+
+end
