src/compiler_generic/toy_example/embedding/core/Floor1_access.thy
@@ -1,0 +1,712 @@
+(*****************************************************************************
+ * Featherweight-OCL --- A Formal Semantics for UML-OCL Version OCL 2.5
+ *                       for the OMG Standard.
+ *                       http://www.brucker.ch/projects/hol-testgen/
+ *
+ * Floor1_access.thy ---
+ * This file is part of HOL-TestGen.
+ *
+ * Copyright (c) 2013-2015 Université Paris-Sud, France
+ *               2013-2015 IRT SystemX, France
+ *
+ * All rights reserved.
+ *
+ * Redistribution and use in source and binary forms, with or without
+ * modification, are permitted provided that the following conditions are
+ * met:
+ *
+ *     * Redistributions of source code must retain the above copyright
+ *       notice, this list of conditions and the following disclaimer.
+ *
+ *     * Redistributions in binary form must reproduce the above
+ *       copyright notice, this list of conditions and the following
+ *       disclaimer in the documentation and/or other materials provided
+ *       with the distribution.
+ *
+ *     * Neither the name of the copyright holders nor the names of its
+ *       contributors may be used to endorse or promote products derived
+ *       from this software without specific prior written permission.
+ *
+ * THIS SOFTWARE IS PROVIDED BY THE COPYRIGHT HOLDERS AND CONTRIBUTORS
+ * "AS IS" AND ANY EXPRESS OR IMPLIED WARRANTIES, INCLUDING, BUT NOT
+ * LIMITED TO, THE IMPLIED WARRANTIES OF MERCHANTABILITY AND FITNESS FOR
+ * A PARTICULAR PURPOSE ARE DISCLAIMED. IN NO EVENT SHALL THE COPYRIGHT
+ * OWNER OR CONTRIBUTORS BE LIABLE FOR ANY DIRECT, INDIRECT, INCIDENTAL,
+ * SPECIAL, EXEMPLARY, OR CONSEQUENTIAL DAMAGES (INCLUDING, BUT NOT
+ * LIMITED TO, PROCUREMENT OF SUBSTITUTE GOODS OR SERVICES; LOSS OF USE,
+ * DATA, OR PROFITS; OR BUSINESS INTERRUPTION) HOWEVER CAUSED AND ON ANY
+ * THEORY OF LIABILITY, WHETHER IN CONTRACT, STRICT LIABILITY, OR TORT
+ * (INCLUDING NEGLIGENCE OR OTHERWISE) ARISING IN ANY WAY OUT OF THE USE
+ * OF THIS SOFTWARE, EVEN IF ADVISED OF THE POSSIBILITY OF SUCH DAMAGE.
+ ******************************************************************************)
+(* $Id:$ *)
+
+header{* Part ... *}
+
+theory  Floor1_access
+imports Core_init
+begin
+
+section{* Translation of AST *}
+
+subsection{* accessors *}
+
+definition "print_access_oid_uniq_gen Thy_def D_ocl_oid_start_upd def_rewrite =
+  (\<lambda>expr ocl.
+      (\<lambda>(l, oid_start). (L.map Thy_def l, D_ocl_oid_start_upd ocl oid_start))
+      (let (l, (acc, _)) = fold_class (\<lambda>isub_name name l_attr l_inh _ _ cpt.
+         let l_inh = L.map (\<lambda> OclClass _ l _ \<Rightarrow> l) (of_inh l_inh) in
+         let (l, cpt) = L.mapM (L.mapM
+           (\<lambda> (attr, OclTy_object (OclTyObj (OclTyCore ty_obj) _)) \<Rightarrow>
+                                            (let\<^sub>O\<^sub>C\<^sub>a\<^sub>m\<^sub>l obj_oid = TyObj_ass_id ty_obj
+                                               ; obj_name_from_nat = TyObjN_ass_switch (TyObj_from ty_obj) in \<lambda>(cpt, rbt) \<Rightarrow>
+             let (cpt_obj, cpt_rbt) =
+               case RBT.lookup rbt obj_oid of
+                 None \<Rightarrow> (cpt, oidSucAssoc cpt, RBT.insert obj_oid cpt rbt)
+               | Some cpt_obj \<Rightarrow> (cpt_obj, cpt, rbt) in
+             ( [def_rewrite obj_name_from_nat name isub_name attr (oidGetAssoc cpt_obj)]
+             , cpt_rbt))
+            | _ \<Rightarrow> \<lambda>cpt. ([], cpt)))
+           (l_attr # l_inh) cpt in
+         (L.flatten (L.flatten l), cpt)) (D_ocl_oid_start ocl, RBT.empty) expr in
+       (L.flatten l, acc)))"
+definition "print_access_oid_uniq_ml =
+  print_access_oid_uniq_gen
+    O.ML
+    (\<lambda>x _. x)
+    (\<lambda>obj_name_from_nat name _ attr cpt_obj.
+      SML (SML.rewrite_val
+                   (SML.basic [print_access_oid_uniq_mlname obj_name_from_nat name attr])
+                   \<open>=\<close>
+                   (SML.oid \<open>\<close> cpt_obj)))"
+definition "print_access_oid_uniq =
+  print_access_oid_uniq_gen
+    O.definition
+    (\<lambda>ocl oid_start. ocl \<lparr> D_ocl_oid_start := oid_start \<rparr>)
+    (\<lambda>obj_name_from_nat _ isub_name attr cpt_obj.
+      Definition (Expr_rewrite
+                   (Expr_basic [print_access_oid_uniq_name obj_name_from_nat isub_name attr])
+                   \<open>=\<close>
+                   (Expr_oid \<open>\<close> cpt_obj)))"
+
+definition "print_access_eval_extract _ = start_map O.definition
+  (let lets = \<lambda>var def. Definition (Expr_rewrite (Expr_basic [var]) \<open>=\<close> def)
+     ; a = \<lambda>f x. Expr_app f [x]
+     ; b = \<lambda>s. Expr_basic [s] in
+  [ let\<^sub>O\<^sub>C\<^sub>a\<^sub>m\<^sub>l var_x = \<open>x\<close>
+      ; var_f = \<open>f\<close>
+      ; some_some = (\<lambda>x. Expr_some (Expr_some x))
+      ; var_obj = \<open>obj\<close> in
+    Definition (Expr_rewrite
+                  (Expr_basic [var_eval_extract, var_x, var_f])
+                  \<open>=\<close>
+                  (Expr_lam \<open>\<tau>\<close>
+                     (\<lambda>var_tau. Expr_case (Expr_basic [var_x, var_tau])
+                     [ (some_some (Expr_basic [var_obj]), Expr_app var_f [Expr_app \<open>oid_of\<close> [Expr_basic [var_obj]], Expr_basic [var_tau]])
+                     , (Expr_basic [wildcard], Expr_basic [\<open>invalid\<close>, var_tau])])))
+  , lets var_in_pre_state (b \<open>fst\<close>)
+  , lets var_in_post_state (b \<open>snd\<close>)
+  , lets var_reconst_basetype Expr_basety
+  , let\<^sub>O\<^sub>C\<^sub>a\<^sub>m\<^sub>l var_x = \<open>x\<close> in
+     Definition (Expr_rewrite (Expr_basic [var_reconst_basetype_void, var_x])
+                              \<open>=\<close>
+                              (Expr_binop (Expr_basic [var_Abs_Void]) \<open>o\<close> (a var_reconst_basetype (b var_x)))) ])"
+
+
+definition "print_access_choose_switch
+              lets mk_var expr
+              print_access_choose_n
+              sexpr_list sexpr_function sexpr_pair =
+  L.flatten
+       (L.map
+          (\<lambda>n.
+           let l = L.upto 0 (n - 1) in
+           L.map (let l = sexpr_list (L.map mk_var l) in (\<lambda>(i,j).
+             (lets
+                (print_access_choose_n n i j)
+                (sexpr_function [(l, (sexpr_pair (mk_var i) (mk_var j)))]))))
+             ((L.flatten o L.flatten) (L.map (\<lambda>i. L.map (\<lambda>j. if i = j then [] else [(i, j)]) l) l)))
+          (class_arity expr))"
+definition "print_access_choose_ml = start_map'''' O.ML o (\<lambda>expr _.
+  (let a = \<lambda>f x. SML.apply f [x]
+     ; b = \<lambda>s. SML.basic [s]
+     ; lets = \<lambda>var exp. SML (SML.rewrite_val (SML.basic [var]) \<open>=\<close> exp)
+     ; mk_var = \<lambda>i. b (S.flatten [\<open>x\<close>, String.of_natural i]) in
+   L.flatten
+   [ print_access_choose_switch
+       lets mk_var expr
+       print_access_choose_mlname
+       SML.list SML.function SML.pair ]))"
+definition "print_access_choose = start_map'''' O.definition o (\<lambda>expr _.
+  (let a = \<lambda>f x. Expr_app f [x]
+     ; b = \<lambda>s. Expr_basic [s]
+     ; lets = \<lambda>var exp. Definition (Expr_rewrite (Expr_basic [var]) \<open>=\<close> exp)
+     ; lets' = \<lambda>\<^sub>S\<^sub>c\<^sub>a\<^sub>l\<^sub>avar exp. Definition (Expr_rewrite (Expr_basic [var]) \<open>=\<close> (b exp))
+     ; lets'' = \<lambda>\<^sub>S\<^sub>c\<^sub>a\<^sub>l\<^sub>avar exp. Definition (Expr_rewrite (Expr_basic [var]) \<open>=\<close> (Expr_lam \<open>l\<close> (\<lambda>var_l. Expr_binop (b var_l) \<open>!\<close> (b exp))))
+     ; _(* ignored *) = 
+        let l_flatten = \<open>L.flatten\<close> in
+        [ lets l_flatten (let fun_foldl = \<lambda>f base.
+                             Expr_lam \<open>l\<close> (\<lambda>var_l. Expr_app \<open>foldl\<close> [Expr_lam \<open>acc\<close> f, base, a \<open>rev\<close> (b var_l)]) in
+                           fun_foldl (\<lambda>var_acc.
+                             fun_foldl (\<lambda>var_acc.
+                               Expr_lam \<open>l\<close> (\<lambda>var_l. Expr_app \<open>Cons\<close> (L.map b [var_l, var_acc]))) (b var_acc)) (b \<open>Nil\<close>))
+        , lets var_map_of_list (Expr_app \<open>foldl\<close>
+            [ Expr_lam \<open>map\<close> (\<lambda>var_map.
+                let var_x = \<open>x\<close>
+                  ; var_l0 = \<open>l0\<close>
+                  ; var_l1 = \<open>l1\<close>
+                  ; f_map = a var_map in
+                Expr_lambdas0 (Expr_pair (b var_x) (b var_l1))
+                  (Expr_case (f_map (b var_x))
+                    (L.map (\<lambda>(pat, e). (pat, f_map (Expr_binop (b var_x) \<open>\<mapsto>\<close> e)))
+                      [ (b \<open>None\<close>, b var_l1)
+                      , (Expr_some (b var_l0), a l_flatten (Expr_list (L.map b [var_l0, var_l1])))])))
+            , b \<open>Map.empty\<close>])] in
+  L.flatten
+  [ let\<^sub>O\<^sub>C\<^sub>a\<^sub>m\<^sub>l a = \<lambda>f x. Expr_app f [x]
+      ; b = \<lambda>s. Expr_basic [s]
+      ; lets = \<lambda>var exp. Definition (Expr_rewrite (Expr_basic [var]) \<open>=\<close> exp)
+      ; mk_var = \<lambda>i. b (S.flatten [\<open>x\<close>, String.of_natural i]) in
+    print_access_choose_switch
+      lets mk_var expr
+      print_access_choose_name
+      Expr_list Expr_function Expr_pair
+  , []] ))"
+
+definition "print_access_deref_oid_name isub_name = isub_name var_deref_oid"
+definition "print_access_deref_oid = start_map O.definition o
+  map_class (\<lambda>isub_name _ _ _ _ _.
+    let var_fs = \<open>fst_snd\<close>
+      ; var_f = \<open>f\<close>
+      ; var_oid = \<open>oid\<close>
+      ; var_obj = \<open>obj\<close> in
+    Definition (Expr_rewrite
+                  (Expr_basic [print_access_deref_oid_name isub_name, var_fs, var_f, var_oid])
+                  \<open>=\<close>
+                  (Expr_lam \<open>\<tau>\<close>
+                     (\<lambda>var_tau. Expr_case (Expr_app \<open>heap\<close> [Expr_basic [var_fs, var_tau], Expr_basic [var_oid]])
+                     [ (Expr_some (Expr_basic [isub_name datatype_in, var_obj]), Expr_basic [var_f, var_obj, var_tau])
+                     , (Expr_basic [wildcard], Expr_basic [\<open>invalid\<close>, var_tau]) ]))))"
+
+definition "print_access_deref_assocs_name' name_from isub_name isup_attr =
+  S.flatten [var_deref, \<open>_\<close>, isub_name var_assocs, \<open>_\<close>, String.of_natural name_from, isup_attr \<open>_\<close>]"
+definition "print_access_deref_assocs_name name_from isub_name attr =
+  print_access_deref_assocs_name' name_from isub_name (\<lambda>s. s @@ String.isup attr)"
+definition "print_access_deref_assocs = start_map'''' O.definition o (\<lambda>expr design_analysis.
+  (if design_analysis = Gen_only_design then \<lambda>_. [] else (\<lambda>expr. L.flatten (L.flatten (map_class (\<lambda>isub_name name l_attr l_inherited _ _.
+  let l_inherited = map_class_inh l_inherited in
+  let var_fst_snd = \<open>fst_snd\<close>
+    ; var_f = \<open>f\<close>
+    ; b = \<lambda>s. Expr_basic [s] in
+    L.flatten (L.map (L.map
+      (\<lambda> (attr, OclTy_object (OclTyObj (OclTyCore ty_obj) _)) \<Rightarrow>
+           let name_from = TyObjN_ass_switch (TyObj_from ty_obj) in
+           [Definition (Expr_rewrite
+                  (Expr_basic [print_access_deref_assocs_name name_from isub_name attr, var_fst_snd, var_f])
+                  \<open>=\<close>
+                  (Expr_binop
+                    (Expr_app
+                      var_deref_assocs
+                        (L.map b [ var_fst_snd
+                               , print_access_choose_name (TyObj_ass_arity ty_obj) name_from (TyObjN_ass_switch (TyObj_to ty_obj))
+                               , print_access_oid_uniq_name name_from isub_name attr
+                               , var_f ]))
+                    \<open>\<circ>\<close>
+                    (b \<open>oid_of\<close>)))]
+       | _ \<Rightarrow> []))
+      (l_attr # l_inherited))) expr)))) expr)"
+
+definition "print_access_select_name isup_attr isub_name = isup_attr (isub_name var_select)"
+definition "print_access_select = start_map'' O.definition o (\<lambda>expr base_attr _ base_attr''.
+  let b = \<lambda>s. Expr_basic [s] in
+  map_class_arg_only0 (\<lambda>isub_name name l_attr.
+    let l_attr = base_attr l_attr in
+    let var_f = \<open>f\<close>
+      ; wildc = Expr_basic [wildcard] in
+    let (_, _, l) = (foldl
+      (\<lambda>(l_wildl, l_wildr, l_acc) (attr, _).
+        let isup_attr = (\<lambda>s. s @@ String.isup attr) in
+        ( wildc # l_wildl
+        , tl l_wildr
+        , Definition (Expr_rewrite
+                       (Expr_basic [print_access_select_name isup_attr isub_name, var_f])
+                       \<open>=\<close>
+                       (let var_attr = b (\<open>x_\<close> @@ String.isup attr) in
+                        Expr_function
+                          (L.map (\<lambda>(lhs,rhs). ( Expr_app
+                                                         (isub_name datatype_constr_name)
+                                                         ( wildc
+                                                         # L.flatten [l_wildl, [lhs], l_wildr])
+                                                     , rhs))
+                            [ ( Expr_basic [\<open>\<bottom>\<close>], Expr_basic [\<open>null\<close>] )
+                            , ( Expr_some var_attr
+                              , Expr_app var_f [var_attr]) ]))) # l_acc))
+      ([], L.map (\<lambda>_. wildc) (tl l_attr), [])
+      l_attr) in
+    rev l)
+  (\<lambda>isub_name name (l_attr, l_inherited, l_cons).
+    let l_inherited = L.flatten (L.map (\<lambda> OclClass _ l _ \<Rightarrow> l) (of_inh l_inherited)) in
+    let (l_attr, l_inherited) = base_attr'' (l_attr, l_inherited) in
+    let var_f = \<open>f\<close>
+      ; wildc = Expr_basic [wildcard] in
+    let (_, _, l) = (foldl
+      (\<lambda>(l_wildl, l_wildr, l_acc) (attr, _).
+        let isup_attr = (\<lambda>s. s @@ String.isup attr) in
+        ( wildc # l_wildl
+        , tl l_wildr
+        , Definition (Expr_rewrite
+                       (Expr_basic [isup_attr (isub_name var_select), var_f])
+                       \<open>=\<close>
+                       (let var_attr = b (\<open>x_\<close> @@ String.isup attr) in
+                        Expr_function
+                          (L.flatten (L.map (\<lambda>(lhs,rhs). ( Expr_app
+                                                         (isub_name datatype_constr_name)
+                                                         ( Expr_app (isub_name datatype_ext_constr_name)
+                                                             (wildc # L.flatten [l_wildl, [lhs], l_wildr])
+                                                         # L.map (\<lambda>_. wildc) l_attr)
+                                                     , rhs))
+                            [ ( Expr_basic [\<open>\<bottom>\<close>], Expr_basic [\<open>null\<close>] )
+                            , ( Expr_some var_attr
+                              , Expr_app var_f [var_attr]) ]
+                            # (L.map (\<lambda> OclClass x _ _ \<Rightarrow> let var_x = String.lowercase x in
+                                             (Expr_app
+                                                         (isub_name datatype_constr_name)
+                                                         ( Expr_app (datatype_ext_constr_name @@ mk_constr_name name x)
+                                                             [Expr_basic [var_x]]
+                                                         # L.map (\<lambda>_. wildc) l_attr), (Expr_app (isup_attr (var_select @@ String.isub x))
+                                                                                                     (L.map (\<lambda>x. Expr_basic [x]) [var_f, var_x]) ))) (of_sub l_cons))
+                            # [])))) # l_acc))
+      ([], L.map (\<lambda>_. wildc) (tl l_inherited), [])
+      l_inherited) in
+    rev l) expr)"
+
+definition "print_access_select_obj_name' isub_name attr = isub_name var_select @@ attr"
+definition "print_access_select_obj_name isub_name attr = print_access_select_obj_name' isub_name (String.isup attr)"
+definition "print_access_select_obj = start_map'''' O.definition o (\<lambda>expr design_analysis.
+  (if design_analysis = Gen_only_design then \<lambda>_. [] else (\<lambda>expr. L.flatten (L.flatten (map_class (\<lambda>isub_name name l_attr l_inh _ _.
+    let l_inh = map_class_inh l_inh in
+    L.flatten (fst (L.mapM (L.mapM
+      (\<lambda> (attr, OclTy_object (OclTyObj (OclTyCore ty_obj) _)) \<Rightarrow> \<lambda>rbt.
+          if lookup2 rbt (name, attr) = None then
+           ( [ Definition
+                (let b = \<lambda>s. Expr_basic [s] in
+                 Expr_rewrite
+                  (b (isub_name var_select @@ String.isup attr))
+                  \<open>=\<close>
+                  (b (let\<^sub>O\<^sub>C\<^sub>a\<^sub>m\<^sub>l obj_mult = TyObjN_role_multip (TyObj_to ty_obj) in
+                      case (is_sequence obj_mult, single_multip obj_mult) of
+                        (True, True) \<Rightarrow> var_select_object_sequence_any
+                      | (True, False) \<Rightarrow> var_select_object_sequence
+                      | (False, True) \<Rightarrow> var_select_object_set_any
+                      | (False, False) \<Rightarrow> var_select_object_set)))]
+           , insert2 (name, attr) () rbt)
+         else ([], rbt)
+       | _ \<Rightarrow> Pair []))
+      (l_attr # l_inh) RBT.empty))) expr)))) expr)"
+
+definition "print_access_dot_consts =
+ (L.mapM (\<lambda>(f_update, x) ocl. (O.consts x, ocl \<lparr> D_ocl_accessor := f_update (D_ocl_accessor ocl) \<rparr> ))) o
+  (L.flatten o L.flatten o map_class (\<lambda>isub_name name l_attr _ _ _.
+    L.map (\<lambda>(attr_n, attr_ty).
+      L.map
+        (\<lambda>(var_at_when_hol, var_at_when_ocl, f_update_ocl).
+          let name =
+             S.flatten [ \<open>dot\<close>
+                     , case attr_ty of
+                         OclTy_object (OclTyObj (OclTyCore ty_obj) _) \<Rightarrow> S.flatten [\<open>_\<close>, String.of_natural (TyObjN_ass_switch (TyObj_from ty_obj)), \<open>_\<close>]
+                       | _ \<Rightarrow> \<open>\<close>
+                     , String.isup attr_n, var_at_when_hol] in
+          ( f_update_ocl (\<lambda> l. String.to_String\<^sub>b\<^sub>a\<^sub>s\<^sub>e name # l)
+          , Consts_raw0
+            name
+            (Ty_arrow
+              (Ty_apply (Ty_base \<open>val\<close>) [Ty_base \<open>\<AA>\<close>, Ty_base \<open>'\<alpha>\<close>])
+              (print_access_dot_consts_ty attr_ty))
+            (let dot_name = mk_dot attr_n var_at_when_ocl
+               ; mk_par = \<lambda>s1 s2. S.flatten [s1, \<open> '/* \<close>, s2, \<open> *'/\<close>] in
+             case attr_ty of OclTy_object (OclTyObj (OclTyCore ty_obj) _) \<Rightarrow>
+               (case apply_optim_ass_arity
+                       ty_obj
+                       (mk_par
+                          dot_name
+                          (let\<^sub>O\<^sub>C\<^sub>a\<^sub>m\<^sub>l ty_obj = TyObj_from ty_obj in
+                           case TyObjN_role_name ty_obj of
+                                None => String.of_natural (TyObjN_ass_switch ty_obj)
+                              | Some s => s)) of
+                  None \<Rightarrow> dot_name
+                | Some dot_name \<Rightarrow> dot_name)
+                           | _ \<Rightarrow> dot_name)
+            None))
+        [ (var_at_when_hol_post, var_at_when_ocl_post, update_D_ocl_accessor_post)
+        , (var_at_when_hol_pre, var_at_when_ocl_pre, update_D_ocl_accessor_pre)]) l_attr))"
+
+definition "print_access_dot_name isub_name dot_at_when attr_ty isup_attr =
+  S.flatten [ isup_attr (let dot_name = isub_name \<open>dot\<close> in
+                       case attr_ty of
+                         OclTy_object (OclTyObj (OclTyCore ty_obj) _) \<Rightarrow> S.flatten [dot_name, \<open>_\<close>, String.of_natural (TyObjN_ass_switch (TyObj_from ty_obj)), \<open>_\<close>]
+                       | _ \<Rightarrow> dot_name)
+          , dot_at_when]"
+
+fun print_access_dot_aux where
+   "print_access_dot_aux deref_oid x =
+    (\<lambda> OclTy_collection c ty \<Rightarrow>
+         Expr_app (if is_sequence c then var_select_object_sequence else var_select_object_set)
+                    [print_access_dot_aux deref_oid ty]
+     | OclTy_pair ty1 ty2 \<Rightarrow> Expr_app var_select_object_pair [print_access_dot_aux deref_oid ty1, print_access_dot_aux deref_oid ty2]
+     | OclTy_object (OclTyObj (OclTyCore_pre s) _) \<Rightarrow> deref_oid (Some s) [Expr_basic [var_reconst_basetype]]
+     | OclTy_base_void \<Rightarrow> Expr_basic [var_reconst_basetype_void]
+     | _ \<Rightarrow> Expr_basic [var_reconst_basetype]) x"
+
+definition "print_access_dot = start_map'''' O.defs o (\<lambda>expr design_analysis.
+  map_class_arg_only_var'
+    (\<lambda>isub_name name (var_in_when_state, dot_at_when) attr_ty isup_attr dot_attr.
+            [ Defs_overloaded
+                (print_access_dot_name isub_name dot_at_when attr_ty isup_attr)
+                (let var_x = \<open>x\<close> in
+                 Expr_rewrite
+                   (dot_attr (Expr_annot_ocl (Expr_basic [var_x]) name))
+                   \<open>\<equiv>\<close>
+                   (Expr_app var_eval_extract [Expr_basic [var_x],
+                    let deref_oid = \<lambda>attr_orig l. Expr_app (case attr_orig of None \<Rightarrow> isub_name var_deref_oid
+                                                                              | Some orig_n \<Rightarrow> var_deref_oid @@ String.isub orig_n) (Expr_basic [var_in_when_state] # l) in
+                    deref_oid None
+                      [ ( case attr_ty of
+                            OclTy_object (OclTyObj (OclTyCore ty_obj) _) \<Rightarrow>
+                              if design_analysis = Gen_only_design then id else
+                                (\<lambda>l. Expr_app (print_access_deref_assocs_name' (TyObjN_ass_switch (TyObj_from ty_obj)) isub_name isup_attr) (Expr_basic [var_in_when_state] # [l]))
+                          | _ \<Rightarrow> id)
+                          (Expr_app (isup_attr (isub_name var_select))
+                            [case attr_ty of
+                               OclTy_raw _ \<Rightarrow> Expr_basic [var_reconst_basetype]
+                             | OclTy_object (OclTyObj (OclTyCore ty_obj) _) \<Rightarrow>
+                                 let ty_obj = TyObj_to ty_obj
+                                   ; der_name = deref_oid (Some (TyObjN_role_ty ty_obj)) [Expr_basic [var_reconst_basetype]] in
+                                 if design_analysis = Gen_only_design then
+                                   let obj_mult = TyObjN_role_multip ty_obj
+                                     ; (var_select_object_name_any, var_select_object_name) =
+                                         if is_sequence obj_mult then
+                                           (var_select_object_sequence_any, var_select_object_sequence)
+                                         else
+                                           (var_select_object_set_any, var_select_object_set) in
+                                   Expr_app (if single_multip obj_mult then
+                                                 var_select_object_name_any
+                                               else
+                                                 var_select_object_name) [der_name]
+                                 else
+                                   der_name
+                             | x \<Rightarrow> print_access_dot_aux deref_oid x ]) ] ])) ]) expr)"
+
+definition "print_access_dot_lemmas_id_set =
+  (if activate_simp_optimization then
+     map_class_arg_only_var'
+       (\<lambda>isub_name _ (_, dot_at_when) attr_ty isup_attr _. [print_access_dot_name isub_name dot_at_when attr_ty isup_attr])
+   else (\<lambda>_. []))"
+
+definition "print_access_dot_lemmas_id_name = \<open>dot_accessor\<close>"
+definition "print_access_dot_lemmas_id = start_map' (\<lambda>expr.
+       (let name_set = print_access_dot_lemmas_id_set expr in
+       case name_set of [] \<Rightarrow> [] | _ \<Rightarrow> L.map O.lemmas
+         [ Lemmas_nosimp print_access_dot_lemmas_id_name (L.map T.thm name_set) ]))"
+
+definition "print_access_dot_cp_lemmas_set =
+  (if activate_simp_optimization then [hol_definition var_eval_extract] else [])"
+
+definition "print_access_dot_cp_lemmas = start_map' (\<lambda>_.
+  L.map (\<lambda>x. O.lemmas (Lemmas_simp \<open>\<close> [T.thm x])) print_access_dot_cp_lemmas_set)"
+
+definition "print_access_dot_lemma_cp_name isub_name dot_at_when attr_ty isup_attr = S.flatten [\<open>cp_\<close>, print_access_dot_name isub_name dot_at_when attr_ty isup_attr]"
+definition "print_access_dot_lemma_cp = start_map O.lemma o
+ (let auto = \<lambda>l. M.auto_simp_add2 [T.thms print_access_dot_lemmas_id_name] (L.map hol_definition (\<open>cp\<close> # l)) in
+  map_class_arg_only_var
+    (\<lambda>isub_name name (_, dot_at_when) attr_ty isup_attr dot_attr.
+            [ Lemma
+                (print_access_dot_lemma_cp_name isub_name dot_at_when attr_ty isup_attr)
+                [Expr_app \<open>cp\<close> [Expr_lam \<open>X\<close> (\<lambda>var_x. dot_attr (Expr_annot_ocl (Expr_basic [var_x]) name)) ]]
+                []
+                (C.by [auto (if print_access_dot_cp_lemmas_set = [] then
+                                  [var_eval_extract, S.flatten [isup_attr (isub_name \<open>dot\<close>), dot_at_when]]
+                                else
+                                  [])]) ])
+    (\<lambda>isub_name name (_, dot_at_when) attr_ty isup_attr dot_attr.
+            [ Lemma
+                (print_access_dot_lemma_cp_name isub_name dot_at_when attr_ty isup_attr)
+                [Expr_app \<open>cp\<close> [Expr_lam \<open>X\<close> (\<lambda>var_x. dot_attr (Expr_annot_ocl (Expr_basic [var_x]) name)) ]]
+                []
+                (if print_access_dot_cp_lemmas_set = [] then C.sorry (* fold l_hierarchy, take only subclass, unfold the corresponding definition *)
+                 else C.by [auto []]) ]))"
+
+definition "print_access_dot_lemmas_cp = start_map O.lemmas o (\<lambda>expr.
+  case map_class_arg_only_var'
+    (\<lambda>isub_name _ (_, dot_at_when) attr_ty isup_attr _.
+      [T.thm (print_access_dot_lemma_cp_name isub_name dot_at_when attr_ty isup_attr) ])
+    expr
+  of [] \<Rightarrow> []
+   | l \<Rightarrow> [Lemmas_simp \<open>\<close> l])"
+
+definition "print_access_lemma_strict_name isub_name dot_at_when attr_ty isup_attr name_invalid = S.flatten [print_access_dot_name isub_name dot_at_when attr_ty isup_attr, \<open>_\<close>, name_invalid]"
+definition "print_access_lemma_strict expr = (start_map O.lemma o
+  map_class_arg_only_var' (\<lambda>isub_name name (_, dot_at_when) attr_ty isup_attr dot_attr.
+            L.map (\<lambda>(name_invalid, meth_invalid). Lemma
+                  (print_access_lemma_strict_name isub_name dot_at_when attr_ty isup_attr name_invalid)
+                  [Expr_rewrite
+                     (dot_attr (Expr_annot_ocl (Expr_basic [name_invalid]) name))
+                     \<open>=\<close>
+                     (Expr_basic [\<open>invalid\<close>])]
+                  []
+                  (if print_access_dot_lemmas_id_set expr = [] | print_access_dot_cp_lemmas_set = [] then
+                     C.sorry else
+                   C.by [ M.rule (T.thm \<open>ext\<close>),
+                             M.simp_add2 [T.thms print_access_dot_lemmas_id_name]
+                                           (L.map hol_definition
+                                             (let l = (let l = (\<open>bot_option\<close> # meth_invalid) in
+                                              if print_access_dot_lemmas_id_set expr = [] then
+                                                S.flatten [isup_attr (isub_name \<open>dot\<close>), dot_at_when] # l
+                                              else l) in
+                                              if print_access_dot_cp_lemmas_set = []
+                                              then
+                                                \<open>eval_extract\<close> # l
+                                              else l))]) )
+                [(\<open>invalid\<close>, [\<open>invalid\<close>]), (\<open>null\<close>, [\<open>null_fun\<close>, \<open>null_option\<close>])])) expr"
+
+definition "print_access_def_mono_name isub_name dot_at_when attr_ty isup_attr =
+  S.flatten [ \<open>defined_mono_\<close>, print_access_dot_name isub_name dot_at_when attr_ty isup_attr ]"
+definition "print_access_def_mono = start_map'''' O.lemma o (\<lambda>expr _.
+  map_class_arg_only_var'
+    (\<lambda>isub_name name (_, dot_at_when) attr_ty isup_attr dot_attr.
+      let var_X = \<open>X\<close>
+        ; var_tau = \<open>\<tau>\<close>
+        ; a = \<lambda>f x. Expr_app f [x]
+        ; b = \<lambda>s. Expr_basic [s]
+        ; f0 = \<lambda>e. Expr_binop (Expr_basic [var_tau]) \<open>\<Turnstile>\<close> e
+        ; f = \<lambda>e. f0 (Expr_app \<open>\<delta>\<close> [e]) in
+            [ Lemma
+                (print_access_def_mono_name isub_name dot_at_when attr_ty isup_attr)
+                (L.map f [ dot_attr (Expr_annot_ocl (b var_X) name)
+                            , b var_X ])
+                (let\<^sub>O\<^sub>C\<^sub>a\<^sub>m\<^sub>l f_tac = \<lambda>s.
+                   [ M.case_tac (f0 (Expr_warning_parenthesis (Expr_rewrite (b var_X) \<open>\<triangleq>\<close> (b s))))
+                   , M.insert [T.where (T.thm \<open>StrongEq_L_subst2\<close>)
+                                           [ (\<open>P\<close>, Expr_lam \<open>x\<close> (\<lambda>var_X. a \<open>\<delta>\<close> (dot_attr (b var_X))))
+                                           , (\<open>\<tau>\<close>, b \<open>\<tau>\<close>)
+                                           , (\<open>x\<close>, b var_X)
+                                           , (\<open>y\<close>, b s)]]
+                   , M.simp_add [ \<open>foundation16'\<close>
+                                  , print_access_lemma_strict_name isub_name dot_at_when attr_ty isup_attr s] ] in
+                 [ f_tac \<open>invalid\<close>
+                 , f_tac \<open>null\<close> ])
+                (C.by [M.simp_add [\<open>defined_split\<close>]]) ]) expr)"
+
+definition "print_access_is_repr_name isub_name dot_at_when attr_ty isup_attr =
+  S.flatten [ \<open>is_repr_\<close>, print_access_dot_name isub_name dot_at_when attr_ty isup_attr ]"
+definition "print_access_is_repr = start_map'''' O.lemma o (\<lambda>expr design_analysis.
+ (let is_design = design_analysis = Gen_only_design
+    ; App_a = \<lambda>l. C.apply (if is_design then [] else l)
+    ; App_d = \<lambda>l. C.apply (if is_design then l else []) in
+  map_class_arg_only_var'
+    (\<lambda>isub_name name (var_in_when_state, dot_at_when) attr_ty isup_attr dot_attr.
+      case attr_ty of OclTy_object (OclTyObj (OclTyCore ty_obj) _) \<Rightarrow>
+     (let ty_mult = TyObjN_role_multip (TyObj_to ty_obj) in
+      if single_multip ty_mult then
+      let var_X = \<open>X\<close>
+        ; var_tau = \<open>\<tau>\<close>
+        ; var_def_dot = \<open>def_dot\<close>
+        ; a = \<lambda>f x. Expr_app f [x]
+        ; ap = \<lambda>f x. Expr_applys (Expr_pat f) [x]
+        ; ap' = \<lambda>f x. Expr_applys (Expr_pat f) x
+        ; b = \<lambda>s. Expr_basic [s]
+        ; f0 = \<lambda>e. Expr_binop (Expr_basic [var_tau]) \<open>\<Turnstile>\<close> e
+        ; f = \<lambda>e. f0 (Expr_app \<open>\<delta>\<close> [e])
+        ; attr_ty' = is_sequence ty_mult
+        ; name_from = TyObjN_ass_switch (TyObj_from ty_obj)
+        ; name_to = TyObjN_role_ty (TyObj_to ty_obj)
+        ; isub_name_to = \<lambda>s. s @@ String.isub name_to in
+            [ Lemma_assumes
+                (print_access_is_repr_name isub_name dot_at_when attr_ty isup_attr)
+                [ (var_def_dot, False, f (dot_attr (Expr_annot_ocl (b var_X) name))) ]
+                (Expr_app \<open>is_represented_in_state\<close> [b var_in_when_state, dot_attr (Expr_basic [var_X]), b name_to, b var_tau])
+(let\<^sub>O\<^sub>C\<^sub>a\<^sub>m\<^sub>l (* existential variables *)
+     v_a0 = \<open>a0\<close>
+   ; v_a = \<open>a\<close>
+   ; v_b = \<open>b\<close>
+   ; v_r = \<open>r\<close>
+   ; v_typeoid = \<open>typeoid\<close>
+   ; v_opt = \<open>opt\<close>
+   ; v_aa = \<open>aa\<close>
+   ; v_e = \<open>e\<close>
+   ; v_aaa = \<open>aaa\<close>
+
+     (* schematic variables *)
+   ; vs_t = \<open>t\<close>
+   ; vs_sel_any = \<open>sel_any\<close>
+
+     (* *)
+   ; l_thes = \<lambda>l. Some (l @@@@ [Expr_pat \<open>thesis\<close>])
+   ; l_thes0 = \<lambda>l. Some (l @@@@ [Expr_pat \<open>t\<close>])
+   ; hol_d = L.map hol_definition
+   ; thol_d = L.map (T.thm o hol_definition)
+   ; App_f = \<lambda>l e. C.fix_let l [] e []
+   ; App_d_f = \<lambda>l e. if is_design then App_f l e else C.apply []
+   ; App_f' = \<lambda>l. C.fix_let l []
+   ; f_ss = \<lambda>v. a \<open>Some\<close> (a \<open>Some\<close> (b v)) in
+ [ C.apply [M.insert [T.simplified (T.OF (T.thm (print_access_def_mono_name isub_name dot_at_when attr_ty isup_attr))
+                                           (T.thm var_def_dot))
+                                   (T.thm \<open>foundation16\<close>)]]
+ , C.apply [M.case_tac (a var_X (b var_tau)), M.simp_add [hol_definition \<open>bot_option\<close>]]
+ (* *)
+ , App_f' [v_a0]
+          (l_thes [ Expr_binop (a var_X (b var_tau)) \<open>\<noteq>\<close> (b \<open>null\<close>)
+                  , Expr_binop (a var_X (b var_tau)) \<open>=\<close> (a \<open>Some\<close> (b v_a0)) ])
+          [C.apply_end [M.simp_all]]
+ , C.apply [M.case_tac (b v_a0), M.simp_add (L.map hol_definition [\<open>null_option\<close>, \<open>bot_option\<close>]), M.clarify]
+ (* *)
+ , App_f [v_a] (l_thes [ Expr_binop (a var_X (b var_tau)) \<open>=\<close> (f_ss v_a) ])
+ , C.apply [M.case_tac (Expr_app \<open>heap\<close> [ a var_in_when_state (b var_tau)
+                                          , a \<open>oid_of\<close> (b v_a)]), M.simp_add (hol_d [\<open>invalid\<close>, \<open>bot_option\<close>])]
+ , C.apply [ M.insert [T.thm \<open>def_dot\<close>]
+       , M.simp_add_split ( T.thm (print_access_dot_name isub_name dot_at_when attr_ty isup_attr)
+                            # thol_d [ \<open>is_represented_in_state\<close>
+                                     , print_access_select_name isup_attr isub_name
+                                     , print_access_deref_oid_name isub_name
+                                     , var_in_when_state
+                                     , \<open>defined\<close>, \<open>OclValid\<close>, \<open>false\<close>, \<open>true\<close>, \<open>invalid\<close>, \<open>bot_fun\<close>])
+                            [T.thm \<open>split_if_asm\<close>]]
+ (* *)
+ , App_f [v_b] (l_thes [ Expr_binop (a var_X (b var_tau)) \<open>=\<close> (f_ss v_a)
+                       , Expr_rewrite (Expr_app \<open>heap\<close> [ a var_in_when_state (b var_tau)
+                                                           , a \<open>oid_of\<close> (b v_a)])
+                                      \<open>=\<close>
+                                      (a \<open>Some\<close> (b v_b)) ])
+ , C.apply [ M.insert [T.simplified (T.thm \<open>def_dot\<close>) (T.thm \<open>foundation16\<close>)]
+       , M.auto_simp_add ( print_access_dot_name isub_name dot_at_when attr_ty isup_attr
+                           # hol_d [ \<open>is_represented_in_state\<close>
+                                   , print_access_deref_oid_name isub_name
+                                   , \<open>bot_option\<close>, \<open>null_option\<close>])]
+ , C.apply [ M.case_tac (b v_b), M.simp_all_add (hol_d [\<open>invalid\<close>, \<open>bot_option\<close>]) ]
+ , App_a [ M.simp_add (hol_d [print_access_deref_assocs_name' name_from isub_name isup_attr, var_deref_assocs]) ]
+ , App_a [ M.case_tac (Expr_app (\<open>assocs\<close>) [ a var_in_when_state (b var_tau)
+                                               , b (print_access_oid_uniq_name' name_from isub_name (isup_attr \<open>\<close>)) ])
+         , M.simp_add (hol_d [\<open>invalid\<close>, \<open>bot_option\<close>])
+         , M.simp_add (hol_d [print_access_select_obj_name' isub_name (isup_attr \<open>\<close>)]) ]
+ (* *)
+ , C.fix_let
+     [v_r, v_typeoid]
+     [ ( Expr_pat vs_t
+       , Expr_rewrite (f_ss v_r) \<open>\<in>\<close> (Expr_binop
+                                              (Expr_parenthesis
+                                                (Expr_binop (b \<open>Some\<close>) \<open>o\<close> (b (print_astype_from_universe_name name_to))))
+                                              \<open>`\<close>
+                                              (a \<open>ran\<close> (a \<open>heap\<close> (a var_in_when_state (b var_tau))))))
+     , ( Expr_pat vs_sel_any
+       , Expr_app (if attr_ty' then var_select_object_sequence_any else var_select_object_set_any)
+                    [ Expr_app (print_access_deref_oid_name isub_name_to) [b var_in_when_state, b var_reconst_basetype] ])]
+     (Some [ Expr_rewrite (if is_design then
+                             Expr_app (print_access_select_name isup_attr isub_name)
+                                      [ Expr_pat vs_sel_any
+                                      , b v_typeoid
+                                      , b var_tau ]
+                           else
+                             Expr_applys (Expr_pat vs_sel_any)
+                                      [ b v_typeoid
+                                      , b var_tau ]) \<open>=\<close> (f_ss v_r)
+           , Expr_pat vs_t ])
+     []
+ , App_d [ M.case_tac (b v_typeoid), M.simp_add (hol_d [print_access_select_name isup_attr isub_name]) ]
+ (* *)
+ , App_d_f [v_opt]
+     (l_thes0
+       [ Expr_rewrite (Expr_applys (Expr_case (b v_opt)
+                                              [ (b \<open>None\<close>, b \<open>null\<close>)
+                                              , let var_x = \<open>x\<close> in
+                                                (a \<open>Some\<close> (b var_x), ap vs_sel_any (b var_x)) ])
+                                   [ b var_tau ])
+                      \<open>=\<close>
+                      (f_ss v_r) ])
+ , App_d [ M.case_tac (b v_opt), M.auto_simp_add (hol_d [\<open>null_fun\<close>, \<open>null_option\<close>, \<open>bot_option\<close>]) ]
+ (* *)
+ , App_f' [v_aa]
+     (l_thes0
+       [ Expr_binop (b var_tau) \<open>\<Turnstile>\<close> (a \<open>\<delta>\<close> (ap vs_sel_any (b v_aa)))
+       , Expr_rewrite (ap' vs_sel_any [ b v_aa, b var_tau ]) \<open>=\<close> (f_ss v_r) ])
+     [ C.apply_end [ M.simp_all_only [] ]
+     , C.apply_end [ M.simp_add (\<open>foundation16\<close> # hol_d [\<open>bot_option\<close>, \<open>null_option\<close>]) ] ]
+ , C.apply [ M.drule (T.simplified (T.thm (if attr_ty' then
+                                               var_select_object_sequence_any_exec
+                                             else
+                                               var_select_object_set_any_exec))
+                                   (T.thm \<open>foundation22\<close>)), M.erule (T.thm \<open>exE\<close>) ]
+ (* *)
+ , App_f' [v_e]
+     (l_thes0
+       [ Expr_rewrite (ap' vs_sel_any [ b v_aa, b var_tau ]) \<open>=\<close> (f_ss v_r)
+       , Expr_rewrite (ap' vs_sel_any [ b v_aa, b var_tau ])
+                      \<open>=\<close>
+                      (Expr_app (print_access_deref_oid_name isub_name_to)
+                                  (L.map b [ var_in_when_state
+                                              , var_reconst_basetype
+                                              , v_e
+                                              , var_tau ])) ])
+     [ C.apply_end [ M.plus [M.blast None] ] ]
+ , C.apply [ M.simp_add (hol_d [print_access_deref_oid_name isub_name_to]) ]
+ , C.apply [ M.case_tac (Expr_app \<open>heap\<close> [ a var_in_when_state (b var_tau), b v_e ])
+       , M.simp_add (hol_d [\<open>invalid\<close>, \<open>bot_option\<close>]), M.simp ]
+ (* *)
+ , App_f [v_aaa]
+     (l_thes0
+       [ Expr_rewrite (Expr_case (b v_aaa)
+                                 [ let\<^sub>O\<^sub>C\<^sub>a\<^sub>m\<^sub>l var_obj = \<open>obj\<close> in
+                                   (a (isub_name_to datatype_in) (b var_obj), Expr_app var_reconst_basetype [b var_obj, b var_tau])
+                                 , (b wildcard, a \<open>invalid\<close> (b var_tau)) ])
+                      \<open>=\<close>
+                      (f_ss v_r)
+       , Expr_rewrite (Expr_app \<open>heap\<close> [ a var_in_when_state (b var_tau), b v_e ])
+                      \<open>=\<close>
+                      (a \<open>Some\<close> (b v_aaa)) ])
+ , C.apply [ M.case_tac (b v_aaa), M.auto_simp_add (hol_d [\<open>invalid\<close>, \<open>bot_option\<close>, \<open>image\<close>, \<open>ran\<close>]) ]
+ , C.apply [ M.rule (T.where (T.thm \<open>exI\<close>) [(\<open>x\<close>, a (isub_name_to datatype_in) (b v_r))])
+       , M.simp_add_split (thol_d [print_astype_from_universe_name name_to, \<open>Let\<close>, var_reconst_basetype])
+                            [T.thm \<open>split_if_asm\<close>] ] ])
+                (C.by [ M.rule' ]) ] else [] (* TODO *))
+      | _ \<Rightarrow> [] (* TODO *))) expr)"
+
+definition "print_access_repr_allinst = start_map''''' O.lemma o (\<lambda>expr (sorry, dirty) design_analysis.
+  if sorry = Some Gen_sorry | sorry = None & dirty then 
+  map_class_arg_only_var'
+    (\<lambda>isub_name name (var_in_when_state, dot_at_when) attr_ty isup_attr dot_attr.
+      case attr_ty of OclTy_object (OclTyObj (OclTyCore ty_obj) _) \<Rightarrow>
+        let var_tau = \<open>\<tau>\<close>
+          ; f = \<lambda>e. Expr_binop (Expr_basic [var_tau]) \<open>\<Turnstile>\<close> e
+          ; a = \<lambda>f x. Expr_app f [x]
+          ; b = \<lambda>s. Expr_basic [s]
+          ; var_x = \<open>x\<close> in
+            [ Lemma
+                (S.flatten [ isup_attr (S.flatten [isub_name \<open>dot_repr\<close>, \<open>_\<close>, String.of_natural (TyObjN_ass_switch (TyObj_from ty_obj)), \<open>_\<close>])
+                         , dot_at_when])
+                ([ f (a \<open>\<delta>\<close> (dot_attr (Expr_annot_ocl (Expr_basic [var_x]) name)))
+                 , let\<^sub>O\<^sub>C\<^sub>a\<^sub>m\<^sub>l all_inst = if var_in_when_state \<triangleq> var_in_pre_state then
+                                        \<open>OclAllInstances_at_pre\<close>
+                                      else
+                                        \<open>OclAllInstances_at_post\<close> in
+                   Expr_binop
+                      (let\<^sub>O\<^sub>C\<^sub>a\<^sub>m\<^sub>l ty_obj = TyObj_to ty_obj
+                         ; name' = TyObjN_role_ty ty_obj
+                         ; obj_mult = TyObjN_role_multip ty_obj in
+                       f (Expr_app
+                            (if single_multip obj_mult then
+                               \<open>UML_Set.OclIncludes\<close>
+                             else
+                               \<open>UML_Set.OclIncludesAll\<close>)
+                            [ a all_inst (b name')
+                            , let\<^sub>O\<^sub>C\<^sub>a\<^sub>m\<^sub>l x = dot_attr (b var_x) in
+                              if is_sequence obj_mult then
+                                a \<open>OclAsSet\<^sub>S\<^sub>e\<^sub>q\<close> x
+                              else
+                                x ]))
+                      \<open>\<and>\<close>
+                      (f (Expr_app \<open>UML_Set.OclIncludes\<close> [ a all_inst (b name)
+                                                           , b var_x ]))])
+                []
+                C.sorry ]
+      | _ \<Rightarrow> []) expr
+  else [])"
+
+end
