src/compiler_generic/toy_example/embedding/meta_toy/Parser_UML.thy
@@ -1,0 +1,322 @@
+(*****************************************************************************
+ * Featherweight-OCL --- A Formal Semantics for UML-OCL Version OCL 2.5
+ *                       for the OMG Standard.
+ *                       http://www.brucker.ch/projects/hol-testgen/
+ *
+ * Parser_UML.thy ---
+ * This file is part of HOL-TestGen.
+ *
+ * Copyright (c) 2013-2015 Université Paris-Sud, France
+ *               2013-2015 IRT SystemX, France
+ *
+ * All rights reserved.
+ *
+ * Redistribution and use in source and binary forms, with or without
+ * modification, are permitted provided that the following conditions are
+ * met:
+ *
+ *     * Redistributions of source code must retain the above copyright
+ *       notice, this list of conditions and the following disclaimer.
+ *
+ *     * Redistributions in binary form must reproduce the above
+ *       copyright notice, this list of conditions and the following
+ *       disclaimer in the documentation and/or other materials provided
+ *       with the distribution.
+ *
+ *     * Neither the name of the copyright holders nor the names of its
+ *       contributors may be used to endorse or promote products derived
+ *       from this software without specific prior written permission.
+ *
+ * THIS SOFTWARE IS PROVIDED BY THE COPYRIGHT HOLDERS AND CONTRIBUTORS
+ * "AS IS" AND ANY EXPRESS OR IMPLIED WARRANTIES, INCLUDING, BUT NOT
+ * LIMITED TO, THE IMPLIED WARRANTIES OF MERCHANTABILITY AND FITNESS FOR
+ * A PARTICULAR PURPOSE ARE DISCLAIMED. IN NO EVENT SHALL THE COPYRIGHT
+ * OWNER OR CONTRIBUTORS BE LIABLE FOR ANY DIRECT, INDIRECT, INCIDENTAL,
+ * SPECIAL, EXEMPLARY, OR CONSEQUENTIAL DAMAGES (INCLUDING, BUT NOT
+ * LIMITED TO, PROCUREMENT OF SUBSTITUTE GOODS OR SERVICES; LOSS OF USE,
+ * DATA, OR PROFITS; OR BUSINESS INTERRUPTION) HOWEVER CAUSED AND ON ANY
+ * THEORY OF LIABILITY, WHETHER IN CONTRACT, STRICT LIABILITY, OR TORT
+ * (INCLUDING NEGLIGENCE OR OTHERWISE) ARISING IN ANY WAY OUT OF THE USE
+ * OF THIS SOFTWARE, EVEN IF ADVISED OF THE POSSIBILITY OF SUCH DAMAGE.
+ ******************************************************************************)
+(* $Id:$ *)
+
+header{* Part ... *}
+
+theory  Parser_UML
+imports Meta_UML
+        "../../../meta_isabelle/Parser_Pure"
+begin
+
+section{* Generation to both Form (setup part) *}
+
+definition "ocl_multiplicity_rec0 f ocl = f
+  (TyMult ocl)
+  (TyRole ocl)
+  (TyCollect ocl)"
+
+definition "ocl_multiplicity_rec f ocl = ocl_multiplicity_rec0 f ocl
+  (ocl_multiplicity.more ocl)"
+
+definition "ocl_ty_class_node_rec0 f ocl = f
+  (TyObjN_ass_switch ocl)
+  (TyObjN_role_multip ocl)
+  (TyObjN_role_ty ocl)"
+
+definition "ocl_ty_class_node_rec f ocl = ocl_ty_class_node_rec0 f ocl
+  (ocl_ty_class_node.more ocl)"
+
+definition "ocl_ty_class_rec0 f ocl = f
+  (TyObj_name ocl)
+  (TyObj_ass_id ocl)
+  (TyObj_ass_arity ocl)
+  (TyObj_from ocl)
+  (TyObj_to ocl)"
+
+definition "ocl_ty_class_rec f ocl = ocl_ty_class_rec0 f ocl
+  (ocl_ty_class.more ocl)"
+
+definition "ocl_class_raw_rec0 f ocl = f
+  (ClassRaw_name ocl)
+  (ClassRaw_own ocl)
+  (ClassRaw_clause ocl)
+  (ClassRaw_abstract ocl)"
+
+definition "ocl_class_raw_rec f ocl = ocl_class_raw_rec0 f ocl
+  (ocl_class_raw.more ocl)"
+
+definition "ocl_association_rec0 f ocl = f
+  (OclAss_type ocl)
+  (OclAss_relation ocl)"
+
+definition "ocl_association_rec f ocl = ocl_association_rec0 f ocl
+  (ocl_association.more ocl)"
+
+definition "ocl_ctxt_pre_post_rec0 f ocl = f
+  (Ctxt_fun_name ocl)
+  (Ctxt_fun_ty ocl)
+  (Ctxt_expr ocl)"
+
+definition "ocl_ctxt_pre_post_rec f ocl = ocl_ctxt_pre_post_rec0 f ocl
+  (ocl_ctxt_pre_post.more ocl)"
+
+definition "ocl_ctxt_rec0 f ocl = f
+  (Ctxt_param ocl)
+  (Ctxt_ty ocl)
+  (Ctxt_clause ocl)"
+
+definition "ocl_ctxt_rec f ocl = ocl_ctxt_rec0 f ocl
+  (ocl_ctxt.more ocl)"
+
+(* *)
+
+lemma [code]: "ocl_class_raw.extend = (\<lambda>ocl v. ocl_class_raw_rec0 (co4 (\<lambda>f. f v) ocl_class_raw_ext) ocl)"
+by(intro ext, simp add: ocl_class_raw_rec0_def
+                        ocl_class_raw.extend_def
+                        co4_def K_def)
+lemma [code]: "ocl_class_raw.make = co4 (\<lambda>f. f ()) ocl_class_raw_ext"
+by(intro ext, simp add: ocl_class_raw.make_def
+                        co4_def)
+lemma [code]: "ocl_class_raw.truncate = ocl_class_raw_rec (co4 K ocl_class_raw.make)"
+by(intro ext, simp add: ocl_class_raw_rec0_def
+                        ocl_class_raw_rec_def
+                        ocl_class_raw.truncate_def
+                        ocl_class_raw.make_def
+                        co4_def K_def)
+
+lemma [code]: "ocl_association.extend = (\<lambda>ocl v. ocl_association_rec0 (co2 (\<lambda>f. f v) ocl_association_ext) ocl)"
+by(intro ext, simp add: ocl_association_rec0_def
+                        ocl_association.extend_def
+                        co2_def K_def)
+lemma [code]: "ocl_association.make = co2 (\<lambda>f. f ()) ocl_association_ext"
+by(intro ext, simp add: ocl_association.make_def
+                        co2_def)
+lemma [code]: "ocl_association.truncate = ocl_association_rec (co2 K ocl_association.make)"
+by(intro ext, simp add: ocl_association_rec0_def
+                        ocl_association_rec_def
+                        ocl_association.truncate_def
+                        ocl_association.make_def
+                        co2_def K_def)
+
+subsection{* i of ... *} (* i_of *)
+
+subsubsection{* general *}
+
+context i_of
+begin
+
+definition "i_of_ocl_collection b = rec_ocl_collection
+  (b \<open>Set\<close>)
+  (b \<open>Sequence\<close>)
+  (b \<open>Ordered0\<close>)
+  (b \<open>Subsets0\<close>)
+  (b \<open>Union0\<close>)
+  (b \<open>Redefines0\<close>)
+  (b \<open>Derived0\<close>)
+  (b \<open>Qualifier0\<close>)
+  (b \<open>Nonunique0\<close>)"
+
+definition "i_of_ocl_multiplicity_single a b = rec_ocl_multiplicity_single
+  (ap1 a (b \<open>Mult_nat\<close>) (i_of_nat a b))
+  (b \<open>Mult_star\<close>)
+  (b \<open>Mult_infinity\<close>)"
+
+definition "i_of_ocl_multiplicity a b f = ocl_multiplicity_rec
+  (ap4 a (b (ext \<open>ocl_multiplicity_ext\<close>))
+    (i_of_list a b (i_of_pair a b (i_of_ocl_multiplicity_single a b) (i_of_option a b (i_of_ocl_multiplicity_single a b))))
+    (i_of_option a b (i_of_string a b))
+    (i_of_list a b (i_of_ocl_collection b))
+    (f a b))"
+
+definition "i_of_ocl_ty_class_node a b f = ocl_ty_class_node_rec
+  (ap4 a (b (ext \<open>ocl_ty_class_node_ext\<close>))
+    (i_of_nat a b)
+    (i_of_ocl_multiplicity a b (K i_of_unit))
+    (i_of_string a b)
+    (f a b))"
+
+definition "i_of_ocl_ty_class a b f = ocl_ty_class_rec
+  (ap6 a (b (ext \<open>ocl_ty_class_ext\<close>))
+    (i_of_string a b)
+    (i_of_nat a b)
+    (i_of_nat a b)
+    (i_of_ocl_ty_class_node a b (K i_of_unit))
+    (i_of_ocl_ty_class_node a b (K i_of_unit))
+    (f a b))"
+
+definition "i_of_ocl_ty_obj_core a b = rec_ocl_ty_obj_core
+  (ap1 a (b \<open>OclTyCore_pre\<close>) (i_of_string a b))
+  (ap1 a (b \<open>OclTyCore\<close>) (i_of_ocl_ty_class a b (K i_of_unit)))"
+
+definition "i_of_ocl_ty_obj a b = rec_ocl_ty_obj
+  (ap2 a (b \<open>OclTyObj\<close>) (i_of_ocl_ty_obj_core a b) (i_of_list a b (i_of_list a b (i_of_ocl_ty_obj_core a b))))"
+
+definition "i_of_ocl_ty a b = (\<lambda>f1 f2 f3 f4 f5 f6 f7 f8 f9 f10 f11 f12 f13 f14 f15.
+                                    rec_ocl_ty f1 f2 f3 f4 f5 f6
+                                               f7 (K o f8) (\<lambda>_ _. f9) (f10 o map_prod id snd) (\<lambda>_ _. f11) f12 f13 f14 f15)
+  (b \<open>OclTy_base_void\<close>)
+  (b \<open>OclTy_base_boolean\<close>)
+  (b \<open>OclTy_base_integer\<close>)
+  (b \<open>OclTy_base_unlimitednatural\<close>)
+  (b \<open>OclTy_base_real\<close>)
+  (b \<open>OclTy_base_string\<close>)
+  (ap1 a (b \<open>OclTy_object\<close>) (i_of_ocl_ty_obj a b))
+  (ar2 a (b \<open>OclTy_collection\<close>) (i_of_ocl_multiplicity a b (K i_of_unit)))
+  (ar2 a (b \<open>OclTy_pair\<close>) id)
+  (ap1 a (b \<open>OclTy_binding\<close>) (i_of_pair a b (i_of_option a b (i_of_string a b)) id))
+  (ar2 a (b \<open>OclTy_arrow\<close>) id)
+  (ap1 a (b \<open>OclTy_class_syn\<close>) (i_of_string a b))
+  (ap1 a (b \<open>OclTy_enum\<close>) (i_of_string a b))
+  (ap1 a (b \<open>OclTy_raw\<close>) (i_of_string a b))"
+
+definition "i_of_ocl_association_type a b = rec_ocl_association_type
+  (b \<open>OclAssTy_native_attribute\<close>)
+  (b \<open>OclAssTy_association\<close>)
+  (b \<open>OclAssTy_composition\<close>)
+  (b \<open>OclAssTy_aggregation\<close>)"
+
+definition "i_of_ocl_association_relation a b = rec_ocl_association_relation
+  (ap1 a (b \<open>OclAssRel\<close>)
+    (i_of_list a b (i_of_pair a b (i_of_ocl_ty_obj a b) (i_of_ocl_multiplicity a b (K i_of_unit)))))"
+
+definition "i_of_ocl_association a b f = ocl_association_rec
+  (ap3 a (b (ext \<open>ocl_association_ext\<close>))
+    (i_of_ocl_association_type a b)
+    (i_of_ocl_association_relation a b)
+    (f a b))"
+
+definition "i_of_ocl_ctxt_prefix a b = rec_ocl_ctxt_prefix
+  (b \<open>OclCtxtPre\<close>)
+  (b \<open>OclCtxtPost\<close>)"
+
+definition "i_of_ocl_ctxt_term a b = (\<lambda>f0 f1 f2. rec_ocl_ctxt_term f0 f1 (co1 K f2))
+  (ap1 a (b \<open>T_pure\<close>) (i_of_pure_term a b))
+  (ap2 a (b \<open>T_to_be_parsed\<close>) (i_of_string a b) (i_of_string a b))
+  (ar2 a (b \<open>T_lambda\<close>) (i_of_string a b))"
+
+definition "i_of_ocl_prop a b = rec_ocl_prop
+  (ap2 a (b \<open>OclProp_ctxt\<close>) (i_of_option a b (i_of_string a b)) (i_of_ocl_ctxt_term a b))"
+
+definition "i_of_ocl_ctxt_term_inv a b = rec_ocl_ctxt_term_inv
+  (ap2 a (b \<open>T_inv\<close>) (i_of_bool b) (i_of_ocl_prop a b))"
+
+definition "i_of_ocl_ctxt_term_pp a b = rec_ocl_ctxt_term_pp
+  (ap2 a (b \<open>T_pp\<close>) (i_of_ocl_ctxt_prefix a b) (i_of_ocl_prop a b))
+  (ap1 a (b \<open>T_invariant\<close>) (i_of_ocl_ctxt_term_inv a b))"
+
+definition "i_of_ocl_ctxt_pre_post a b f = ocl_ctxt_pre_post_rec
+  (ap4 a (b (ext \<open>ocl_ctxt_pre_post_ext\<close>))
+    (i_of_string a b)
+    (i_of_ocl_ty a b)
+    (i_of_list a b (i_of_ocl_ctxt_term_pp a b))
+    (f a b))"
+
+definition "i_of_ocl_ctxt_clause a b = rec_ocl_ctxt_clause
+  (ap1 a (b \<open>Ctxt_pp\<close>) (i_of_ocl_ctxt_pre_post a b (K i_of_unit)))
+  (ap1 a (b \<open>Ctxt_inv\<close>) (i_of_ocl_ctxt_term_inv a b))"
+
+definition "i_of_ocl_ctxt a b f = ocl_ctxt_rec
+  (ap4 a (b (ext \<open>ocl_ctxt_ext\<close>))
+    (i_of_list a b (i_of_string a b))
+    (i_of_ocl_ty_obj a b)
+    (i_of_list a b (i_of_ocl_ctxt_clause a b))
+    (f a b))"
+
+definition "i_of_ocl_class a b = (\<lambda>f0 f1 f2 f3. rec_ocl_class (ap3 a f0 f1 f2 f3))
+  (b \<open>OclClass\<close>)
+    (i_of_string a b)
+    (i_of_list a b (i_of_pair a b (i_of_string a b) (i_of_ocl_ty a b)))
+    (i_of_list a b snd)"
+
+definition "i_of_ocl_class_raw a b f = ocl_class_raw_rec
+  (ap5 a (b (ext \<open>ocl_class_raw_ext\<close>))
+    (i_of_ocl_ty_obj a b)
+    (i_of_list a b (i_of_pair a b (i_of_string a b) (i_of_ocl_ty a b)))
+    (i_of_list a b (i_of_ocl_ctxt_clause a b))
+    (i_of_bool b)
+    (f a b))"
+
+definition "i_of_ocl_ass_class a b = rec_ocl_ass_class
+  (ap2 a (b \<open>OclAssClass\<close>)
+    (i_of_ocl_association a b (K i_of_unit))
+    (i_of_ocl_class_raw a b (K i_of_unit)))"
+
+definition "i_of_ocl_class_synonym a b = rec_ocl_class_synonym
+  (ap2 a (b \<open>OclClassSynonym\<close>)
+    (i_of_string a b)
+    (i_of_ocl_ty a b))"
+
+definition "i_of_ocl_enum a b = rec_ocl_enum
+  (ap2 a (b \<open>OclEnum\<close>)
+    (i_of_string a b)
+    (i_of_list a b (i_of_string a b)))"
+
+end
+
+lemmas [code] =
+  i_of.i_of_ocl_collection_def
+  i_of.i_of_ocl_multiplicity_single_def
+  i_of.i_of_ocl_multiplicity_def
+  i_of.i_of_ocl_ty_class_node_def
+  i_of.i_of_ocl_ty_class_def
+  i_of.i_of_ocl_ty_obj_core_def
+  i_of.i_of_ocl_ty_obj_def
+  i_of.i_of_ocl_ty_def
+  i_of.i_of_ocl_association_type_def
+  i_of.i_of_ocl_association_relation_def
+  i_of.i_of_ocl_association_def
+  i_of.i_of_ocl_ctxt_prefix_def
+  i_of.i_of_ocl_ctxt_term_def
+  i_of.i_of_ocl_prop_def
+  i_of.i_of_ocl_ctxt_term_inv_def
+  i_of.i_of_ocl_ctxt_term_pp_def
+  i_of.i_of_ocl_ctxt_pre_post_def
+  i_of.i_of_ocl_ctxt_clause_def
+  i_of.i_of_ocl_ctxt_def
+  i_of.i_of_ocl_class_def
+  i_of.i_of_ocl_class_raw_def
+  i_of.i_of_ocl_ass_class_def
+  i_of.i_of_ocl_class_synonym_def
+  i_of.i_of_ocl_enum_def
+
+end
